Added documentation, small renaming

Code/Prelude/Basics.v
@@ -1,3 +1,9 @@
+Require Import List.
+Require Import Bool.
+Require Import String.
+
+(** * Basics functions *)
+
 Arguments id {_} _/.
 
 Definition comp
@@ -11,13 +17,15 @@ Definition comp
 Notation "g 'o' f" := (comp g f) (at level 40, left associativity).
 Arguments comp {_ _ _} _ _ _/.
 
-(** Facts on decidable equality *)
+(** * Decidable propositions *)
 Inductive dec (A : Prop) : Type :=
-| yes : A -> dec A
-| no : ~A -> dec A.
+| Yes : A -> dec A
+| No : ~A -> dec A.
 
-Arguments yes {_} _.
-Arguments no {_} _.
+Arguments Yes {_} _.
+Arguments No {_} _.
+
+(** * Decidable equality *)
 
 Class decEq (A : Type) :=
   {
@@ -28,7 +36,7 @@ Notation "! p" := (eq_sym p) (at level 80).
 
 Definition transport
            {A : Type}
-           (Y : A -> Prop)
+           (Y : A -> Type)
            {a₁ a₂ : A}
            (p : a₁ = a₂)
   : Y a₁ -> Y a₂
@@ -36,16 +44,45 @@ Definition transport
      | eq_refl => fun z => z
      end.
 
+(* begin hide *)
+Lemma transport_sym_p
+      {A : Type}
+      (B : A -> Type)
+      {x y : A}
+      (p : x = y)
+      (b : B x)
+  : transport B (eq_sym p) (transport B p b) = b.
+Proof.
+  subst.
+  cbn.
+  reflexivity.
+Qed.
+(* end hide *)
+
 (** The unit type has decidable equality *)
 Definition dec_eq_unit
            (x y : unit)
   : dec (x = y)
   := match x , y with
-     | tt , tt => yes eq_refl
+     | tt , tt => Yes eq_refl
      end.
 
 Global Instance decEq_unit : decEq unit
   := {| dec_eq := dec_eq_unit |}.
+
+(** The booleans have decidable equality *)
+Definition dec_eq_bool
+           (x y : bool)
+  : dec (x = y)
+  := match x , y with
+     | true , true => Yes eq_refl
+     | false , false => Yes eq_refl
+     | true , false => No diff_true_false
+     | false , true => No diff_false_true
+     end.
+
+Global Instance decEq_bool : decEq bool
+  := {| dec_eq := dec_eq_bool |}.
 
 (** The product of types with decidable equality has decidable equality *)
 Section ProductDecEq.
@@ -67,14 +104,14 @@ Section ProductDecEq.
              (x y : A * B)
     : dec (x = y)
     := match x , y with
-       | (x₁ , x₂) , (y₁ , y₂) =>
-         match dec_eq x₁ y₁ with
-         | yes p =>
-           match dec_eq x₂ y₂ with
-           | yes q => yes (path_pair p q)
-           | no q => no (fun (r : (x₁ , x₂) = (y₁ , y₂)) => q (f_equal snd r))
+       | (x1 , x2) , (y1 , y2) =>
+         match dec_eq x1 y1 with
+         | Yes p =>
+           match dec_eq x2 y2 with
+           | Yes q => Yes (path_pair p q)
+           | No q => No (fun (r : (x1 , x2) = (y1 , y2)) => q (f_equal snd r))
            end
-         | no p => no (fun (r : (x₁ , x₂) = (y₁ , y₂)) => p (f_equal fst r))
+         | No p => No (fun (r : (x1 , x2) = (y1 , y2)) => p (f_equal fst r))
          end
        end.
 
@@ -88,6 +125,7 @@ Section SumDecEq.
           `{decEq A}
           `{decEq B}.
 
+  (* begin hide *)
   Definition inl_inj
              {x y : A}
              (p : (inl x : A + B) = inl y)
@@ -123,6 +161,7 @@ Section SumDecEq.
   Proof.
     discriminate.
   Qed.
+  (* end hide *)
   
   Definition dec_eq_sum
              (x y : A + B)
@@ -130,15 +169,15 @@ Section SumDecEq.
     := match x , y with
        | inl x , inl y =>
          match dec_eq x y with
-         | yes p => yes (f_equal inl p)
-         | no p => no (fun q => p (inl_inj q))
+         | Yes p => Yes (f_equal inl p)
+         | No p => No (fun q => p (inl_inj q))
          end
-       | inl x , inr y => no (fun q => inl_not_inr q)
-       | inr x , inl y => no (fun q => inr_not_inl q)
+       | inl x , inr y => No (fun q => inl_not_inr q)
+       | inr x , inl y => No (fun q => inr_not_inl q)
        | inr x , inr y =>
          match dec_eq x y with
-         | yes p => yes (f_equal inr p)
-         | no p => no (fun q => p (inr_inj q))
+         | Yes p => Yes (f_equal inr p)
+         | No p => No (fun q => p (inr_inj q))
          end
        end.
 
@@ -148,6 +187,7 @@ End SumDecEq.
 
 
 (** The natural numbers have decidable equality *)
+(* begin hide *)
 Definition help_fam
            (n : nat)
   : Prop
@@ -164,6 +204,7 @@ Proof.
   inversion p.
   reflexivity.
 Qed.
+(* end hide *)
 
 Fixpoint dec_eq_nat
          (n : nat)
@@ -172,17 +213,17 @@ Fixpoint dec_eq_nat
      | 0 =>
        fun m =>
          match m with
-         | 0 => yes eq_refl
-         | S m => no (fun (q : 0 = S m) => transport help_fam q I)
+         | 0 => Yes eq_refl
+         | S m => No (fun (q : 0 = S m) => transport help_fam q I)
          end
      | S n =>
        fun m =>
          match m with
-         | 0 => no (fun (q : S n = 0) => transport help_fam (!q) I)
+         | 0 => No (fun (q : S n = 0) => transport help_fam (!q) I)
          | S m =>
            match dec_eq_nat n m with
-           | yes p => yes (f_equal S p)
-           | no p => no (fun q => p (S_inj q))
+           | Yes p => Yes (f_equal S p)
+           | No p => No (fun q => p (S_inj q))
            end
          end
      end.
@@ -190,3 +231,229 @@ Fixpoint dec_eq_nat
 Global Instance decEq_nat : decEq nat
   := {| dec_eq := dec_eq_nat |}.
 
+(** Strings have decidable equality *)
+Definition dec_eq_string
+           (s1 s2 : string)
+  : dec (s1 = s2)
+  := match string_dec s1 s2 with
+     | left p => Yes p
+     | right p => No p
+     end.
+
+Global Instance decEq_string : decEq string
+  := {| dec_eq := dec_eq_string |}.
+
+(** * Finite types *)
+Class isFinite (A : Type) :=
+  {
+    els : list A ;
+    allIsMember : forall (a : A), In a els
+  }.
+
+(** The unit type is finite *)
+Global Instance isFinite_unit : isFinite unit.
+Proof.
+  simple refine {| els := tt :: nil ; allIsMember := _ |}.
+  intro x.
+  induction x.
+  left.
+  reflexivity.
+Defined.
+
+(** THe booleans are finite *)
+Global Instance isFinite_bool : isFinite bool.
+Proof.
+  simple refine {| els := true :: false :: nil ; allIsMember := _ |}.
+  intros [ | ].
+  - left.
+    reflexivity.
+  - right ; left.
+    reflexivity.
+Defined.
+
+(** The product of finite types is again finite *)
+Fixpoint pairs
+         {A B : Type}
+         (l1 : list A)
+         (l2 : list B)
+  : list (A * B)
+  := match l1 with
+     | nil => nil
+     | (x :: xs) => map (fun b => (x , b)) l2 ++ (pairs xs l2)
+     end.
+
+Proposition in_pairs
+            {A B : Type}
+            (l1 : list A)
+            (l2 : list B)
+            (a : A) (b : B)
+            (Ha : In a l1)
+            (Hb : In b l2)
+  : In (a , b) (pairs l1 l2).
+Proof.
+  induction l1 as [ | x xs IHl ] ; simpl in *.
+  - contradiction.
+  - apply in_or_app.
+    destruct Ha as [Ha | Ha].
+    + left.
+      subst.
+      apply in_map.
+      exact Hb.
+    + right.
+      apply IHl.
+      assumption.
+Qed.      
+
+Global Instance isFinite_prod
+       {A B : Type}
+       `{isFinite A}
+       `{isFinite B}
+  : isFinite (A * B).
+Proof.
+  simple refine {| els := pairs els els ; allIsMember := _ |}.
+  intros [a b].
+  apply in_pairs.
+  - apply allIsMember.
+  - apply allIsMember.
+Defined.
+
+(** The coproduct of finite types is finite *)
+Global Instance isFinite_sum
+       {A B : Type}
+       `{isFinite A}
+       `{isFinite B}
+  : isFinite (A + B).
+Proof.
+  simple refine {| els := map inl els ++ map inr els ;
+                   allIsMember := _ |}.
+  intros [a | b] ; apply in_or_app.
+  - left.
+    apply in_map.
+    apply allIsMember.
+  - right.
+    apply in_map.
+    apply allIsMember.
+Defined.
+
+(** If we have a list, then the type of elements of that list is finite *)
+Inductive members {A : Type} (l : list A) : Type :=
+| MakeMem : forall (x : A), In x l -> members l.
+
+Arguments MakeMem {_ _} _ _.
+
+Program Fixpoint els_members
+        {A : Type}
+        (el_A : list A)
+        (l : list A)
+        (p : forall (a : A), In a l -> In a el_A)
+  : list (members el_A) 
+  := match l with
+     | nil => nil
+     | x :: xs => MakeMem x _ :: els_members el_A xs _
+     end.
+Next Obligation.
+  apply p.
+  left.
+  reflexivity.
+Defined.
+Next Obligation.
+  apply p.
+  right.
+  assumption.
+Defined.
+
+Program Definition A_to_member
+        {A : Type}
+        (el_A : list A)
+        (l : list A)
+        (p : forall (a : A), In a l -> In a el_A)
+        (a : A)
+        (Ha : In a l)
+  : members el_A
+  := MakeMem a _.
+
+Proposition in_els_members
+            {A : Type}
+            (el_A : list A)
+            (l : list A)
+            (p : forall (a : A), In a l -> In a el_A)
+            (a : A)
+            (Ha : In a l)
+  : In (A_to_member el_A l p a Ha) (els_members el_A l p).
+Proof.
+  induction l as [ | x xs IHl].
+  - inversion Ha.
+  - simpl in *.
+    destruct Ha.
+    + left.
+      subst ; reflexivity.
+    + right.
+      apply (IHl (fun a0 H => p a0 (or_intror H))).
+Qed.      
+  
+Global Instance isFinite_members
+       {A : Type}
+       (l : list A)
+  : isFinite (members l).
+Proof.
+  simple refine {| els := els_members l l (fun _ H => H) ;
+                   allIsMember := _ |}.
+  intro x.
+  destruct x.
+  apply (in_els_members l l (fun _ H => H)).
+Defined.
+
+(** * If we have a finite type and a decidable proposition on it, then we can decide whether that proposition holds for every element of that type. *)
+Definition decide_finite_list
+           {A : Type}
+           (P : A -> Prop)
+           (HP : forall (a : A), dec (P a))
+           (l : list A)
+  : dec (forall (a : A), In a l -> P a).
+Proof.
+  induction l as [ | x xs IHl ].
+  - refine (Yes _).
+    intros a q ; simpl in *.
+    contradiction.
+  - destruct (HP x) as [p | p].
+    + destruct IHl as [q | q].
+      * refine (Yes _) ; simpl.
+        intros a Ha.
+        destruct Ha.
+        ** subst.
+           assumption.
+        ** apply q.
+           exact H.
+      * refine (No _).
+        intros n.
+        apply q.
+        intros w Hw.
+        apply n.
+        right.
+        assumption.
+    + refine (No _) ; simpl.
+      intro n.
+      apply p.
+      apply n.
+      left.
+      reflexivity.
+Defined.
+
+Definition decide_finite
+           {A : Type}
+           (P : A -> Prop)
+           (HP : forall (a : A), dec (P a))
+           `{isFinite A}
+  : dec (forall (a : A), P a).
+Proof.
+  destruct (decide_finite_list P HP els) as [p | p].
+  - refine (Yes _).
+    intro a.
+    apply p.
+    apply allIsMember.
+  - refine (No _).
+    intro n.
+    apply p.
+    intros a ?.
+    apply n.
+Defined.
