Code/Syntax/Signature/Contexts.v
@@ -1,8 +1,13 @@
+Require Import Prelude.Basics.
 Require Import Types.
+Require Import Coq.Program.Equality.
+Require Import Eqdep.
 
-Inductive Con (B : Type) : Type :=
-| Empty : Con B
-| Extend : Ty B -> Con B -> Con B.
+(** * Contexts *)
+
+Inductive con (B : Type) : Type :=
+| Empty : con B
+| Extend : ty B -> con B -> con B.
 
 Arguments Empty {_}.
 Arguments Extend {_} _ _.
@@ -10,11 +15,69 @@ Arguments Extend {_} _ _.
 Notation "∙" := Empty : signature.
 Notation "A ,, Γ" := (Extend A Γ) (at level 70, right associativity) : signature.
 
-Inductive Var {B : Type} : Con B -> Ty B -> Type :=
-| Vz : forall (C : Con B) (A : Ty B),
-    Var (A ,, C) A
-| Vs : forall (C : Con B) (A1 A2 : Ty B),
-    Var C A2 -> Var (A1 ,, C) A2.
+(** * Variables *)
+
+(** Note: we represent variables using De Bruijn indices *)
+Inductive var {B : Type} : con B -> ty B -> Type :=
+| Vz : forall (C : con B) (A : ty B),
+    var (A ,, C) A
+| Vs : forall (C : con B) (A1 A2 : ty B),
+    var C A2 -> var (A1 ,, C) A2.
 
 Arguments Vz {_} {_} {_}.
 Arguments Vs {_} {_} {_} {_} _.
+
+(** * Decidable equality of variables *)
+
+(** We decide equality of variables by mapping them to the natural numbers and then deciding equality of the natural numbers. *)
+Fixpoint var_to_nat
+         {B : Type}
+         {C : con B}
+         {A : ty B}
+         (v : var C A)
+  : nat
+  := match v with
+     | Vz => 0
+     | Vs v => S(var_to_nat v)
+     end.
+
+Proposition var_tonat_eq
+            {B : Type}
+            {C : con B}
+            {A : ty B}
+            {v1 v2 : var C A}
+            (p : var_to_nat v1 = var_to_nat v2)
+  : v1 = v2.
+Proof.
+  induction v1.
+  - dependent destruction v2.
+    + reflexivity.
+    + cbn in p.
+      discriminate.
+  - dependent destruction v2.
+    + simpl in p.
+      discriminate.
+    + f_equal.
+      apply IHv1.
+      simpl in p.
+      inversion p.
+      reflexivity.
+Qed.
+
+Definition dec_eq_Var
+        {B : Type}
+        {C : con B}
+        {A : ty B}
+        (v1 v2 : var C A)
+  : dec (v1 = v2)
+  := match dec_eq (var_to_nat v1) (var_to_nat v2) with
+     | Yes p => Yes (var_tonat_eq p)
+     | No p => No (fun q => p (f_equal _ q))
+     end.
+
+Global Instance decEq_Var
+       {B : Type}
+       {C : con B}
+       {A : ty B}
+  : decEq (var C A)
+  := {| dec_eq := dec_eq_Var |}.
