Code/Syntax/Signature/TermSubstitutions.v
@@ -3,70 +3,78 @@ Require Import Syntax.Signature.Contexts.
 Require Import Syntax.Signature.Terms.
 Require Import Syntax.Signature.TermWeakenings.
 
-Inductive Sub {B : Type} {F : Type} : (F -> Ty B) -> Con B -> Con B -> Type :=
-| ToEmpty : forall {ar : F -> Ty B} (C : Con B), Sub ar C ∙
-| ExtendSub : forall {ar : F -> Ty B} {C1 C2 : Con B} {A : Ty B},
-    Sub ar C1 C2 -> Tm ar C1 A -> Sub ar C1 (A ,, C2).
+(** * Substitutions *)
+
+Inductive sub {B : Type} {F : Type} : (F -> ty B) -> con B -> con B -> Type :=
+| ToEmpty : forall {ar : F -> ty B} (C : con B), sub ar C ∙
+| ExtendSub : forall {ar : F -> ty B} {C1 C2 : con B} {A : ty B},
+    sub ar C1 C2 -> tm ar C1 A -> sub ar C1 (A ,, C2).
 
 Notation "s & t" := (ExtendSub s t) (at level 30).
 
+(** * Operations on substitutions *)
+
+(** Dropping a variable *)
 Fixpoint dropSub
          {B : Type}
-         {C1 C2 : Con B}
+         {C1 C2 : con B}
          {F : Type}
-         {ar : F -> Ty B}
-         (A : Ty B)
-         (s : Sub ar C1 C2)
-  : Sub ar (A ,, C1) C2
+         {ar : F -> ty B}
+         (A : ty B)
+         (s : sub ar C1 C2)
+  : sub ar (A ,, C1) C2
   := match s with
      | ToEmpty _ => ToEmpty _
      | s & t => dropSub A s & wkTm t (Drop A (idWk _))
      end.
 
+(** Keeping a variable *)
 Definition keepSub
            {B : Type}
-           {C1 C2 : Con B}
+           {C1 C2 : con B}
            {F : Type}
-           {ar : F -> Ty B}
-           (A : Ty B)
-           (s : Sub ar C1 C2)
-  : Sub ar (A ,, C1) (A ,, C2)
+           {ar : F -> ty B}
+           (A : ty B)
+           (s : sub ar C1 C2)
+  : sub ar (A ,, C1) (A ,, C2)
   := dropSub A s & TmVar Vz.
 
+(** Identity *)
 Fixpoint idSub
          {B : Type}
-         (C : Con B)
+         (C : con B)
          {F : Type}
-         (ar : F -> Ty B)
-         {struct C}
-  : Sub ar C C
+         (ar : F -> ty B)
+  : sub ar C C
   := match C with
      | ∙ => ToEmpty _
      | A ,, C => dropSub A (idSub C ar) & TmVar Vz
      end.
 
+(** Each weakening is a substitution *)
 Fixpoint wkToSub
          {B : Type}
-         {C1 C2 : Con B}
+         {C1 C2 : con B}
          {F : Type}
-         {ar : F -> Ty B}
-         (w : Wk C1 C2)
-  : Sub ar C1 C2
+         {ar : F -> ty B}
+         (w : wk C1 C2)
+  : sub ar C1 C2
   := match w with
      | EmptyWk => ToEmpty ∙
      | Keep A w => keepSub A (wkToSub w)
      | Drop A w => dropSub A (wkToSub w)
      end.
 
+(** * Action of substitution on terms *)
 Definition subVar
            {B : Type}
-           {C1 C2 : Con B}
+           {C1 C2 : con B}
            {F : Type}
-           {ar : F -> Ty B}
-           {A : Ty B}
-           (v : Var C2 A)
-           (s : Sub ar C1 C2)
-  : Tm ar C1 A.
+           {ar : F -> ty B}
+           {A : ty B}
+           (v : var C2 A)
+           (s : sub ar C1 C2)
+  : tm ar C1 A.
 Proof.
   induction s.
   - apply TmVar.
@@ -80,12 +88,12 @@ Defined.
 
 Fixpoint subTm
          {B : Type}
-         {C2 : Con B}
-         {A : Ty B}
+         {C2 : con B}
+         {A : ty B}
          {F : Type}
-         {ar : F -> Ty B}
-         (t : Tm ar C2 A)
-  : forall {C1 : Con B}, Sub ar C1 C2 -> Tm ar C1 A
+         {ar : F -> ty B}
+         (t : tm ar C2 A)
+  : forall {C1 : con B}, sub ar C1 C2 -> tm ar C1 A
   := match t with
      | BaseTm f => fun _ _ => BaseTm f
      | TmVar v => fun _ s => subVar v s
@@ -93,14 +101,15 @@ Fixpoint subTm
      | App f t => fun _ s => App (subTm f s) (subTm t s) 
      end.
 
+(** Composition of substitutions *)
 Definition compSub
            {B : Type}
-           {C1 C2 C3 : Con B}
+           {C1 C2 C3 : con B}
            {F : Type}
-           {ar : F -> Ty B}
-           (s2 : Sub ar C2 C3)
-           (s1 : Sub ar C1 C2)
-  : Sub ar C1 C3.
+           {ar : F -> ty B}
+           (s2 : sub ar C2 C3)
+           (s1 : sub ar C1 C2)
+  : sub ar C1 C3.
 Proof.
   induction s2 as [ | ? ? ? ? s2 IHs2 t ].
   - apply ToEmpty.
