Code/Syntax/Signature/Terms.v
@@ -3,29 +3,16 @@ Require Import Syntax.Signature.Contexts.
 
 Open Scope signature.
 
-(*
-Inductive Tm {B : Type} {F : Type}
-  : (F -> Ty B) -> Con B -> Ty B -> Type
-  :=
-| BaseTm : forall (ar : F -> Ty B) (C : Con B) (f : F),
-    Tm ar C (ar f)
-| TmVar : forall (ar : F -> Ty B) (C : Con B) (A : Ty B),
-    Var C A -> Tm ar C A
-| Lam : forall (ar : F -> Ty B) (C : Con B) (A1 A2 : Ty B),
-    Tm ar (A1 ,, C) A2 -> Tm ar C (A1 ⟶ A2)
-| App : forall (ar : F -> Ty B) (C : Con B) (A1 A2 : Ty B),
-    Tm ar C (A1 ⟶ A2) -> Tm ar C A1 -> Tm ar C A2.
- *)
-
-Inductive Tm {B : Type} {F : Type} (ar : F -> Ty B) (C : Con B) : Ty B -> Type :=
+(** * Terms *)
+Inductive tm {B : Type} {F : Type} (ar : F -> ty B) (C : con B) : ty B -> Type :=
 | BaseTm : forall (f : F),
-    Tm ar C (ar f)
-| TmVar : forall (A : Ty B),
-    Var C A -> Tm ar C A
-| Lam : forall (A1 A2 : Ty B),
-    Tm ar (A1 ,, C) A2 -> Tm ar C (A1 ⟶ A2)
-| App : forall (A1 A2 : Ty B),
-    Tm ar C (A1 ⟶ A2) -> Tm ar C A1 -> Tm ar C A2.
+    tm ar C (ar f)
+| TmVar : forall (A : ty B),
+    var C A -> tm ar C A
+| Lam : forall (A1 A2 : ty B),
+    tm ar (A1 ,, C) A2 -> tm ar C (A1 ⟶ A2)
+| App : forall (A1 A2 : ty B),
+    tm ar C (A1 ⟶ A2) -> tm ar C A1 -> tm ar C A2.
 
 Arguments BaseTm {_} {_} {_} {_} _.
 Arguments TmVar {_} {_} {_} {_} {_} _.
