Code/Syntax/Signature/RewritingSystem.v
@@ -4,83 +4,45 @@ Require Import Syntax.Signature.Terms.
 Require Import Syntax.Signature.TermWeakenings.
 Require Import Syntax.Signature.TermSubstitutions.
 
-(*
-Inductive Rew
-          {B : Type}
-          {F : Type}
-          {ar : F -> Ty B}
-          {R : Type}
-          {Rcon : R -> Con B}
-          {Rtar : R -> B}
-  : forall (lhs rhs : forall (r : R), Tm ar (Rcon r) (Base (Rtar r)))
-           {C : Con B}
-           {A : Ty B},
-    Tm ar C A -> Tm ar C A -> Type
-  :=
-| Trans : forall {lhs rhs : forall (r : R), Tm ar (Rcon r) (Base (Rtar r))}
-                 {C : Con B}
-                 {A : Ty B}
-                 {t1 t2 t3 : Tm ar C A},
-    Rew lhs rhs t1 t2 -> Rew lhs rhs t2 t3 -> Rew lhs rhs t1 t3
-| Rew_App_l : forall {lhs rhs : forall (r : R), Tm ar (Rcon r) (Base (Rtar r))}
-                     {C : Con B}
-                     {A B : Ty B}
-                     {f1 f2 : Tm ar C (A ⟶ B)}
-                     (x : Tm ar C A),
-    Rew lhs rhs f1 f2 -> Rew lhs rhs (f1 · x) (f2 · x)
-| Rew_App_r : forall {lhs rhs : forall (r : R), Tm ar (Rcon r) (Base (Rtar r))}
-                     {C : Con B}
-                     {A B : Ty B}
-                     (f : Tm ar C (A ⟶ B))
-                     {x1 x2 : Tm ar C A},
-    Rew lhs rhs x1 x2 -> Rew lhs rhs (f · x1) (f · x2)
-| Rew_Lam : forall {lhs rhs : forall (r : R), Tm ar (Rcon r) (Base (Rtar r))}
-                   {C : Con B}
-                   {A B : Ty B}
-                   {f1 f2 : Tm ar (A ,, C) B},
-    Rew lhs rhs f1 f2 -> Rew lhs rhs (λ f1) (λ f2)
-| BaseRew : forall {lhs rhs : forall (r : R), Tm ar (Rcon r) (Base (Rtar r))}
-                   {C : Con B}
-                   (r : R)
-                   (s : Sub ar C (Rcon r)),
-    Rew lhs rhs (subTm (lhs r) s) (subTm (rhs r) s).
- *)
+(** * Rewriting systems *)
 
+(** To formulate the beta rule, we need a particular substitution *)
 Definition beta_sub
            {B : Type}
            {F : Type}
-           {ar : F -> Ty B}
-           {C : Con B}
-           {A : Ty B}
-           (t : Tm ar C A)
-  : Sub ar C (A ,, C)
+           {ar : F -> ty B}
+           {C : con B}
+           {A : ty B}
+           (t : tm ar C A)
+  : sub ar C (A ,, C)
   := ExtendSub (idSub C ar) t.
 
-Inductive BetaRed
+(** ** Beta reduction in an AFS *)
+Inductive betaRed
           {B : Type}
           {F : Type}
-          {ar : F -> Ty B}
-          {C : Con B}
-  : forall {A : Ty B}, Tm ar C A -> Tm ar C A -> Prop
+          {ar : F -> ty B}
+          {C : con B}
+  : forall {A : ty B}, tm ar C A -> tm ar C A -> Prop
   :=
-| BetaTrans : forall {A : Ty B}
-                     {t1 t2 t3 : Tm ar C A},
-    BetaRed t1 t2 -> BetaRed t2 t3 -> BetaRed t1 t3
-| BetaRew_App_l : forall {A1 A2 : Ty B}
-                         {f1 f2 : Tm ar C (A1 ⟶ A2)}
-                         (x : Tm ar C A1),
-    BetaRed f1 f2 -> BetaRed (f1 · x) (f2 · x)
-| BetaRew_App_r : forall {A1 A2 : Ty B}
-                         (f : Tm ar C (A1 ⟶ A2))
-                         {x1 x2 : Tm ar C A1},
-    BetaRed x1 x2 -> BetaRed (f · x1) (f · x2)
-| BetaRew_Lam : forall {A1 A2 : Ty B}
-                       {f1 f2 : Tm ar (A1 ,, C) A2},
-    BetaRed f1 f2 -> BetaRed (λ f1) (λ f2)
-| BetaBeta : forall {A1 A2 : Ty B}
-                    (f : Tm ar (A1 ,, C) A2)
-                    (x : Tm ar C A1),
-    BetaRed ((λ f) · x) (subTm f (beta_sub x)).
+| BetaTrans : forall {A : ty B}
+                     {t1 t2 t3 : tm ar C A},
+    betaRed t1 t2 -> betaRed t2 t3 -> betaRed t1 t3
+| BetaRew_App_l : forall {A1 A2 : ty B}
+                         {f1 f2 : tm ar C (A1 ⟶ A2)}
+                         (x : tm ar C A1),
+    betaRed f1 f2 -> betaRed (f1 · x) (f2 · x)
+| BetaRew_App_r : forall {A1 A2 : ty B}
+                         (f : tm ar C (A1 ⟶ A2))
+                         {x1 x2 : tm ar C A1},
+    betaRed x1 x2 -> betaRed (f · x1) (f · x2)
+| BetaRew_Lam : forall {A1 A2 : ty B}
+                       {f1 f2 : tm ar (A1 ,, C) A2},
+    betaRed f1 f2 -> betaRed (λ f1) (λ f2)
+| BetaBeta : forall {A1 A2 : ty B}
+                    (f : tm ar (A1 ,, C) A2)
+                    (x : tm ar C A1),
+    betaRed ((λ f) · x) (subTm f (beta_sub x)).
 
 Arguments BetaTrans {_ _ _ _} {_ _ _ _} _ _.
 Arguments BetaRew_App_l {_ _ _ _} {_ _ _ _} _ _.
@@ -88,38 +50,39 @@ Arguments BetaRew_App_r {_ _ _ _} {_ _} _ {_ _} _.
 Arguments BetaRew_Lam {_ _ _ _} {_ _ _ _} _.
 Arguments BetaBeta {_ _ _ _} {_ _} _ _.
 
-Inductive Rew
+(** ** The rewriting relation in an AFS *)
+Inductive rew
           {B : Type}
           {F : Type}
-          {ar : F -> Ty B}
+          {ar : F -> ty B}
           {R : Type}
-          {Rcon : R -> Con B}
+          {Rcon : R -> con B}
           {Rtar : R -> B}
-          (lhs rhs : forall (r : R), Tm ar (Rcon r) (Base (Rtar r)))
-          {C : Con B}
-  : forall {A : Ty B}, Tm ar C A -> Tm ar C A -> Prop
+          (lhs rhs : forall (r : R), tm ar (Rcon r) (Base (Rtar r)))
+          {C : con B}
+  : forall {A : ty B}, tm ar C A -> tm ar C A -> Prop
   :=
-| Trans : forall {A : Ty B}
-                 {t1 t2 t3 : Tm ar C A},
-    Rew lhs rhs t1 t2 -> Rew lhs rhs t2 t3 -> Rew lhs rhs t1 t3
-| Rew_App_l : forall {A1 A2 : Ty B}
-                     {f1 f2 : Tm ar C (A1 ⟶ A2)}
-                     (x : Tm ar C A1),
-    Rew lhs rhs f1 f2 -> Rew lhs rhs (f1 · x) (f2 · x)
-| Rew_App_r : forall {A1 A2 : Ty B}
-                     (f : Tm ar C (A1 ⟶ A2))
-                     {x1 x2 : Tm ar C A1},
-    Rew lhs rhs x1 x2 -> Rew lhs rhs (f · x1) (f · x2)
-| Rew_Lam : forall {A1 A2 : Ty B}
-                   {f1 f2 : Tm ar (A1 ,, C) A2},
-    Rew lhs rhs f1 f2 -> Rew lhs rhs (λ f1) (λ f2)
-| Beta : forall {A1 A2 : Ty B}
-                (f : Tm ar (A1 ,, C) A2)
-                (x : Tm ar C A1),
-    Rew lhs rhs ((λ f) · x) (subTm f (beta_sub x))
+| Trans : forall {A : ty B}
+                 {t1 t2 t3 : tm ar C A},
+    rew lhs rhs t1 t2 -> rew lhs rhs t2 t3 -> rew lhs rhs t1 t3
+| Rew_App_l : forall {A1 A2 : ty B}
+                     {f1 f2 : tm ar C (A1 ⟶ A2)}
+                     (x : tm ar C A1),
+    rew lhs rhs f1 f2 -> rew lhs rhs (f1 · x) (f2 · x)
+| Rew_App_r : forall {A1 A2 : ty B}
+                     (f : tm ar C (A1 ⟶ A2))
+                     {x1 x2 : tm ar C A1},
+    rew lhs rhs x1 x2 -> rew lhs rhs (f · x1) (f · x2)
+| Rew_Lam : forall {A1 A2 : ty B}
+                   {f1 f2 : tm ar (A1 ,, C) A2},
+    rew lhs rhs f1 f2 -> rew lhs rhs (λ f1) (λ f2)
+| Beta : forall {A1 A2 : ty B}
+                (f : tm ar (A1 ,, C) A2)
+                (x : tm ar C A1),
+    rew lhs rhs ((λ f) · x) (subTm f (beta_sub x))
 | BaseRew : forall (r : R)
-                   (s : Sub ar C (Rcon r)),
-    Rew lhs rhs (subTm (lhs r) s) (subTm (rhs r) s).
+                   (s : sub ar C (Rcon r)),
+    rew lhs rhs (subTm (lhs r) s) (subTm (rhs r) s).
 
 Arguments Trans {_ _ _ _ _ _ _ _ _} {_ _ _ _} _ _.
 Arguments Rew_App_l {_ _ _ _ _ _ _ _ _} {_ _ _ _} _ _.
